src/PlutusIR/Semantics/Static/normaliser/Normalizer_STLC_named.v
@@ -3,7 +3,7 @@ From PlutusCert Require Import STLC_named.
 From PlutusCert Require Import STLC_named_typing.
 From PlutusCert Require Import Normalizer_STLC_DB.
 From PlutusCert Require Import named_DB_iso.
-From PlutusCert Require Import SN_STLC_DB_nd.
+From PlutusCert Require Import SN_F.
 
 Require Import Coq.Lists.List.
 Import ListNotations.
@@ -12,6 +12,6 @@ Import ListNotations.
 Definition normalizer (T : type) (t : term) (H_wt : has_type [] t T) : term :=
   let t_db := toDB t in
   let H_wt_db := toDB_has_type (H_wt) in (* toDB iso preserves well-typedness*)
-  let H_SN := STLC_DB_SN (H_wt_db)  in (* Well typed means strongly normalizing *)
-  let v_db := Normalizer_STLC_DB.normalizer t_db H_SN in
+  let H_SN := strong_normalization (H_wt_db)  in (* Well typed means strongly normalizing *)
+  let v_db := Normalizer_STLC_DB.normalizer (toDB t) H_SN in
   fromDB v_db.
