src/PlutusIR/Semantics/Static/normaliser/SN_F.v
@@ -3,6 +3,7 @@
 From mathcomp Require Import ssreflect ssrbool eqtype ssrnat seq.
 From Coq Require Import ssrfun.
 From PlutusCert Require Import AutosubstSsr ARS normaliser.Context.
+From PlutusCert Require Import STLC_DB STLC_DB_typing.
 
 Set Implicit Arguments.
 Unset Strict Implicit.
@@ -10,18 +11,8 @@ Unset Printing Implicit Defensive.
 
 (** **** Definitions *)
 
-Inductive type : Type :=
-| Base
-| Arr   (A B : type).
-
-Inductive term :=
-| TeVar (x : var)
-| Abs   (A : type) (s : {bind term} )
-| App   (s t : term).
 
 (** **** Substitution Lemmas *)
-
-Global Instance Ids_type : Ids type. unfold Ids. exact (fun s => Base). Defined.
 
 (* Global Instance Rename_type : Rename type. derive. Defined. *)
 
@@ -44,15 +35,15 @@ Global Instance SubstLemmas_term : SubstLemmas term. derive. Qed.
 
 Inductive step : term -> term -> Prop :=
 | step_beta (A : type) (s t : term) :
-    step (App (Abs A s) t) s.[t/]
+    step (tmapp (tmlam A s) t) s.[t/]
 | step_appL s1 s2 t :
-    step s1 s2 -> step (App s1 t) (App s2 t)
+    step s1 s2 -> step (tmapp s1 t) (tmapp s2 t)
 | step_appR s t1 t2 :
-    step t1 t2 -> step (App s t1) (App s t2)
+    step t1 t2 -> step (tmapp s t1) (tmapp s t2)
 | step_abs A s1 s2 :
-    step s1 s2 -> step (Abs A s1) (Abs A s2).
+    step s1 s2 -> step (tmlam A s1) (tmlam A s2).
 
-Lemma step_ebeta A s t u : u = s.[t/] -> step (App (Abs A s) t) u.
+Lemma step_ebeta A s t u : u = s.[t/] -> step (tmapp (tmlam A s) t) u.
 Proof. move->. exact: step_beta. Qed.
 
 Lemma step_subst sigma s t :
@@ -73,14 +64,14 @@ Definition sred sigma tau :=
   forall x : var, red (sigma x) (tau x).
 
 Lemma red_app s1 s2 t1 t2 :
-  red s1 s2 -> red t1 t2 -> red (App s1 t1) (App s2 t2).
+  red s1 s2 -> red t1 t2 -> red (tmapp s1 t1) (tmapp s2 t2).
 Proof.
-  move=> A B. apply: (star_trans (App s2 t1)).
-  - apply: (star_hom (App^~ t1)) A => x y. exact: step_appL.
+  move=> A B. apply: (star_trans (tmapp s2 t1)).
+  - apply: (star_hom (tmapp^~ t1)) A => x y. exact: step_appL.
   - apply: star_hom B => x y. exact: step_appR.
 Qed.
 
-Lemma red_abs A s1 s2 : red s1 s2 -> red (Abs A s1) (Abs A s2).
+Lemma red_abs A s1 s2 : red s1 s2 -> red (tmlam A s1) (tmlam A s2).
 Proof. apply: star_hom => x y. exact: step_abs. Qed.
 
 Lemma red_subst sigma s t : red s t -> red s.[sigma] t.[sigma].
@@ -106,30 +97,14 @@ Qed.
 Lemma red_beta s t1 t2 : step t1 t2 -> red s.[t1/] s.[t2/].
 Proof. move=> h. apply: red_compat => -[|n]/=; [exact: star1|exact: starR]. Qed.
 
-(** **** Syntactic typing *)
-
-Definition ctx := seq type.
-Local Notation "Gamma `_ i" := (get Gamma i) (at level 2).
-
-Inductive has_type (Gamma : ctx) : term -> type -> Prop :=
-| ty_var (x : var) :
-    x < size Gamma -> has_type Gamma (TeVar x) Gamma`_x
-| ty_abs (A B : type) (s : term) :
-    has_type (A :: Gamma) s B ->
-    has_type Gamma (Abs A s) (Arr A B)
-| ty_app (A B : type) (s t : term) :
-    has_type Gamma s (Arr A B) ->
-    has_type Gamma t A ->
-    has_type Gamma (App s t) B.
-
 (* Strong Normalization *)
 
-Notation sn := (sn step).
+Notation SN := (sn step).
 
-Lemma sn_closed t s : sn (App s t) -> sn s.
-Proof. apply: (sn_preimage (h := App^~t)) => x y. exact: step_appL. Qed.
+Lemma sn_closed t s : SN (tmapp s t) -> SN s.
+Proof. apply: (sn_preimage (h := tmapp^~t)) => x y. exact: step_appL. Qed.
 
-Lemma sn_subst sigma s : sn s.[sigma] -> sn s.
+Lemma sn_subst sigma s : SN s.[sigma] -> SN s.
 Proof. apply: sn_preimage => x y. exact: step_subst. Qed.
 
 (* The Reducibility Candidates/Logical Predicate*)
@@ -138,21 +113,24 @@ Definition cand := term -> Prop.
 
 Definition neutral (s : term) : bool :=
   match s with
-    | Abs _ _ => false
+    | tmlam _ _ => false
     | _ => true
   end.
 
 Record reducible (P : cand) : Prop := {
-  p_sn : forall s, P s -> sn s;
+  p_sn : forall s, P s -> SN s;
   p_cl : forall s t, P s -> step s t -> P t;
   p_nc : forall s, neutral s -> (forall t, step s t -> P t) -> P s
 }.
 
 Fixpoint L (T : type) : cand :=
   match T with
-    | Base => sn (** Added base kind! *)
-    | Arr A B => fun s => forall t, L A t -> L B (App s t)
+    | tp_base => SN (** Added base kind! *)
+    | tp_arrow A B => fun s => forall t, L A t -> L B (tmapp s t)
   end.
+
+Global Instance Ids_type : Ids type. unfold Ids. exact (fun s => tp_base). Defined.
+Notation "Gamma `_ i" := (normaliser.Context.get Gamma i) (at level 3).
 
 Definition EL E (sigma : var -> term) : Prop :=
   forall x, x < size E -> L E`_x (sigma x).
@@ -162,11 +140,11 @@ Definition admissible (rho : nat -> cand) :=
 
 (* Facts about reducible sets. *)
 
-Lemma reducible_sn : reducible sn.
+Lemma reducible_sn : reducible SN.
 Proof. constructor; eauto using ARS.sn. by move=> s t [f] /f. Qed.
 Global Hint Resolve reducible_sn : core.
 
-Lemma reducible_var P x : reducible P -> P (TeVar x).
+Lemma reducible_var P x : reducible P -> P (tmvar x).
 Proof. move/p_nc. apply=> // t st. inv st. Qed.
 
 (* Lemma ad_cons P rho :
@@ -179,16 +157,16 @@ Proof with eauto using step.
   elim: A => /=[|A ih1 B ih2].
   - apply reducible_sn.
   - constructor.
-    + move=> s h. apply: (@sn_closed (TeVar 0)). apply: (p_sn (P := L B))...
+    + move=> s h. apply: (@sn_closed (tmvar 0)). apply: (p_sn (P := L B))...
       eapply h. eapply reducible_var; eauto.
-    + move=> s t h st u la. apply: (p_cl _ (s := App s u))...
+    + move=> s t h st u la. apply: (p_cl _ (s := tmapp s u))...
     + move=> s ns h t la.
       have snt := p_sn ih1 la.
       elim: snt la => {} t _ ih3 la. apply: p_nc... move=> v st. inv st=> //...
       apply: ih3 => //. exact: (p_cl ih1) la _.
 Qed.
 
-Corollary L_sn A s : L A s -> sn s.
+Corollary L_sn A s : L A s -> SN s.
 Proof. intros Las. assert (reducible (L A)) by apply (L_reducible A).
    apply (p_sn H). assumption.
 Qed.
@@ -208,7 +186,7 @@ Proof.
   apply (p_nc H); assumption.
 Qed.
 
-Corollary L_var T x : L T (TeVar x).
+Corollary L_var T x : L T (tmvar x).
 Proof.
   apply L_nc; first by []. intros t st. inversion st.
 Qed. 
@@ -224,8 +202,8 @@ Qed.
 (* Closure under beta expansion. *)
 
 Lemma beta_expansion A B s t :
-  sn t -> L A s.[t/] ->
-  L A (App (Abs B s) t).
+  SN t -> L A s.[t/] ->
+  L A (tmapp (tmlam B s) t).
 Proof with eauto.
   move=> snt h. have sns := sn_subst (L_sn h).
   elim: sns t snt h => {} s sns ih1 t. elim=> {} t snt ih2 h.
@@ -237,24 +215,24 @@ Qed.
 (* The fundamental theorem. *)
 
 Theorem soundness Gamma s A :
-  has_type Gamma s A -> forall sigma,
+  has_type_db Gamma s A -> forall sigma,
     EL Gamma sigma -> L A s.[sigma].
 Proof with eauto using L_sn.
   elim=> {Gamma s A} [|Gamma A B s _ ih sigma EL|Gamma A B s t _ ih1 _ ih2 sigma HEL]
-    ;asimpl...
+    ;asimpl...    
   - move=> t h.
     apply: beta_expansion... asimpl. apply: ih... by case.
   - specialize (ih1 _ HEL). specialize (ih2 _ HEL).
     unfold L in ih1. fold L in ih1. apply ih1. apply ih2.
 Qed.
 
-Corollary type_L E s T : has_type E s T -> L T s.
+Corollary type_L E s T : has_type_db E s T -> L T s.
 Proof.
   move=> ty. move: (@soundness E s T ty) => h.
   specialize (h ids). asimpl in h. apply: h => x B. exact: L_var.
 Qed.
 
-Corollary strong_normalization E s T : has_type E s T -> sn s.
+Corollary strong_normalization E s T : has_type_db E s T -> SN s.
 Proof.
   move=>/type_L/L_sn. apply.
 Qed.
