src/PlutusIR/Semantics/Static/normaliser/STLC_DB_typing.v
@@ -1,17 +1,23 @@
-From PlutusCert Require Import STLC_DB.
+From PlutusCert Require Import STLC_DB normaliser.Context.
 Require Import Coq.Strings.String.
 Require Import Coq.Lists.List.
 Import ListNotations.
 Local Open Scope string_scope.
 Local Open Scope list_scope.
+From mathcomp Require Import ssreflect ssrbool eqtype ssrnat seq.
+From PlutusCert Require Import STLC_DB.
 
+Global Instance Ids_type : Ids type. unfold Ids. exact (fun s => tp_base). Defined.
+
+Definition ctx := seq type.
+Notation "Gamma `_ i" := (normaliser.Context.get Gamma i) (at level 3).
 
 (** Kinding of types *)
 Reserved Notation "Δ '|-*db' T ':' K" (at level 40, T at level 0, K at level 0).
-Inductive has_type_db : list type -> term -> type -> Prop :=
-  | K_Var : forall Δ i K,
-      nth_error Δ i = Some K ->
-      Δ |-*db (tmvar i) : K
+Inductive has_type_db : seq type -> term -> type -> Prop :=
+  | K_Var : forall Δ i,
+      i < size Δ ->
+      Δ |-*db (tmvar i) : (Δ`_i)
   | K_Lam : forall Δ K1 T K2,
       (K1 :: Δ) |-*db T : K2 ->
       Δ |-*db (tmlam K1 T) : (tp_arrow K1 K2)
