src/PlutusIR/Semantics/Static/normaliser/Normalisation_STLC_named_sound.v
@@ -1,11 +1,55 @@
 From PlutusCert Require Import Normalisation_STLC_named.
 From PlutusCert Require Import Normalizer_STLC_named.
+From PlutusCert Require Import Normalisation_STLC_DB.
+From PlutusCert Require Import Normalisation_STLC_DB_sound.
+From PlutusCert Require Import named_DB_iso.
+From PlutusCert Require Import STLC_DB_typing.
+From PlutusCert Require Import STLC_named_typing.
+
+Require Import Coq.Strings.String.
+Local Open Scope string_scope.
+Require Import Coq.Lists.List.
+Import ListNotations.
+
+Module N := STLC_named.
+Module D := STLC_DB.
+
+
+(* Uhm, not so easy.
+    For closed terms it should be rather straightforward? 
+    Then you have fromDB (\. t) = \. (fromDB t)?
+    But then how do you prove it by induction?
+    Probably as difficult as SN? *)
+
+(* Other approach? Work through steps? No, for that we need completeness (of DB, so maybe it is possible)*)
+Lemma normaliseDB_then_normalise : forall t_db v_db K,
+    [] |-*db t_db : K -> (* do we need this, and do we need an open environment? *)
+    Normalisation_STLC_DB.normalise t_db v_db -> 
+    Normalisation_STLC_named.normalise (fromDB t_db) (fromDB v_db).
+Proof.
+
+Admitted.
+
+Lemma test : forall t_db v_db,
+    Normalisation_STLC_DB.normalise (toDB t_db) (toDB v_db) ->
+    Normalisation_STLC_named.normalise t_db v_db.
+Proof.
+
+Admitted.
 
 (* Running normalizer on named STLC results in a value that
     satisfies the normalise relation *)
-
 Theorem normalizer_named_sound : forall t T v H_wt,
-    normalizer T t H_wt = v -> normalise t v.
+    Normalizer_STLC_named.normalizer T t H_wt = v -> Normalisation_STLC_named.normalise t v.
 Proof.
     intros t T v H_wt H.
-Admitted.
+    assert (toDB (normalizer T t H_wt) = toDB v).
+    {
+        rewrite H. reflexivity.
+    }
+    unfold normalizer in H0.
+    rewrite named_DB_iso_right in H0.
+    apply normalizer_db_sound in H0.
+    apply test in H0.
+    assumption.
+Qed.
