src/PlutusIR/Semantics/Static/normaliser/Normalizer_STLC_DB2.v
@@ -1,0 +1,222 @@
+From PlutusCert Require Import STLC_named.
+From PlutusCert Require Import Normalisation_STLC_named.
+From PlutusCert Require Import SN_F.
+From PlutusCert Require Import ARS.
+From PlutusCert Require Import named_DB_iso.
+From Autosubst Require Import Autosubst.
+Require Import Coq.Strings.String.
+Require Import Coq.Bool.Bool.
+From Equations Require Import Equations.
+Local Open Scope string_scope.
+Require Import Coq.Lists.List.
+Import ListNotations.
+
+Module N := STLC_named.
+
+(* Monad maybe*)
+(* Define the bind function for option type *)
+Definition bind {A B : Type} (xx : option A) (f : A -> option B) : option B :=
+  match xx with
+  | None => None
+  | Some a => f a
+  end.
+
+(* Define an infix operator for bind *)
+Infix ">>=" := bind (at level 50, left associativity).
+
+Fixpoint namestep (t : term) : option term :=
+    match t with
+    | tmvar X => None
+    | tmapp s t => 
+        if is_normal s then
+            if is_normal t then
+                match s with
+                | tmlam X A s' => Some (substituteTCA X t s')
+                | _ => None
+                end
+            else namestep t >>= fun t' => Some (tmapp s t')
+        else namestep s >>= fun s' => Some (tmapp s' t)
+    | tmlam X A s => (* step' s >>= _ does the normality check for us implicitly*)
+        namestep s >>= fun s' => Some (tmlam X A s')
+    end.
+
+  (* toDB instead of toDB': bad proof smell
+  Exercise to make the problem clear:
+  revAcc : List A -> List A -> List A
+    revAcc [] acc = acc
+    revAcc (x :: xs) acc = revAcc xs (x :: acc)
+
+    reverse : List A -> List A
+    reverse xs = revAcc xs []
+
+    Proving something about reverse often is problematic, you need to prove something over revAcc.
+
+  
+  *)
+
+(* Adding unused free variables to the "toDeBruijn" conversion 
+    preserves stepping
+    This does cause some renaming???
+    *)
+Lemma weaken_fv : forall t t' s fv fv',
+  step (toDB' t fv) (toDB' t' fv') ->
+  step (toDB' t (s:: (List.remove String.string_dec s fv))) (toDB' t' (s:: List.remove String.string_dec s fv')).
+Proof.
+Admitted.
+
+Lemma weaken_fv' : forall t t' ss fv fv',
+  step (toDB' t fv) (toDB' t' fv') ->
+  step (toDB' t (ss ++ fv)) (toDB' t' (ss ++ fv')).
+Proof.
+Admitted.
+
+Lemma weaken_fv'' : forall t t' ss fv fv',
+  step (toDB' t fv) (toDB' t' fv') ->
+  step (toDB' t (fv ++ ss)) (toDB' t' (fv' ++ ss)).
+Proof.
+Admitted.
+
+Lemma step_preserves_freevars : forall t t' fv_t,
+  N.ftv t = fv_t -> namestep t = Some t' -> N.ftv t' = fv_t.
+Proof.
+Admitted.
+
+(* ftv in substTCA x t s never contains "x" (unless t contains "x"???)*)
+Eval compute in (toDB' (N.tmlam "x" tp_base (N.tmvar "z")) ("x"::"y"::["z"])).
+Eval compute in (toDB' (N.tmlam "w" tp_base (N.tmvar "x")) ("x"::["y"])).
+Eval compute in ((D.tmlam D.tp_base (D.tmvar 1)).[D.tmvar 0/]).
+Eval compute in ((D.tmlam D.tp_base (D.tmvar 1)).[(toDB' (N.tmapp (tmvar "y") (tmvar "z")) ["y";"z"])/]).
+Eval compute in ((D.tmlam D.tp_base (D.tmapp (D.tmvar 1) (D.tmvar 8))).[(D.tmvar 12)/]).
+
+
+Lemma uhm2 :
+  substituteTCA "x" (N.tmvar "z") (N.tmlam "y" (N.tp_base) (N.tmapp (N.tmvar "x") (N.tmvar "w"))) = N.tmvar "g".
+
+Lemma uhm :
+  (D.tmlam D.tp_base (D.tmapp (D.tmvar 1) (D.tmvar 8))).[(D.tmvar 12)/] = D.tmvar 1.
+Proof.
+  simpl.
+  unfold up.
+  
+  
+  
+  (* unfold ">>>". *)
+  unfold ".:".
+  unfold ">>>".
+  
+  simpl.
+  
+
+Lemma toDB'subst : forall x t s,
+  toDB' (substituteTCA x t s) (N.ftv (substituteTCA x t s)) = 
+    (toDB' s (x :: List.remove string_dec x (N.ftv (substituteTCA x t s)))).[(toDB' t (N.ftv (substituteTCA x t s)))/].
+Proof.
+  intros x t s.
+  remember (N.ftv (substituteTCA x t s)) as fvs.
+  induction s.
+  - rewrite substituteTCA_equation_1.
+    destruct (x =? s) eqn:Hx; admit.
+   
+Admitted.
+
+(* If a named STLC term steps, then its corresponding DeBruijn term steps*)
+Lemma namestep_implies_step_nd : forall t t',
+  namestep t = Some t' -> 
+  SN_F.step (toDB' t (N.ftv t)) (toDB' t' (N.ftv t')).
+Proof. 
+    (* intros t t' Hns.
+    generalize dependent t'.
+    induction t.
+    - intros t' Hns. discriminate Hns.
+    - intros t' Hns. 
+      inversion Hns.
+      unfold bind in H0.
+      destruct (namestep t0) eqn:Hstep in H0; try discriminate.
+      specialize (IHt t1 Hstep).
+      inversion H0.
+      simpl.
+      apply SN_F.step_abs.
+      apply weaken_fv with (s := s) in IHt.
+      assumption.
+    - intros t' Hns.
+      inversion Hns.
+      destruct (is_normal t1) eqn:Hnorm1.
+      + destruct (is_normal t2) eqn:Hnorm2.
+        * destruct t1 eqn:Ht1; try discriminate.
+          inversion Hnorm1.
+          inversion H0.
+          subst...
+          simpl.
+          remember (List.app (List.remove String.string_dec s (N.ftv t0)) 
+(N.ftv t2)) as fvs.
+          remember (toDB' t0 (s :: fvs)) as t0'.
+          remember (toDB' t2 fvs) as t2'.
+          assert (N.ftv (substituteTCA s t2 t0) = fvs).
+          {
+            admit.
+          }
+          rewrite -> H.
+          assert (toDB' (substituteTCA s t2 t0) fvs = t0'.[t2'/]).
+          {
+            rewrite -> Heqt0'.
+            rewrite -> Heqt2'.
+            rewrite <- H.
+            apply toDB'subst.
+          }
+          rewrite -> H2.
+          apply SN_F.step_beta.
+        * unfold bind in H0.
+          destruct (namestep t2) eqn:Hstep in H0; try discriminate.
+          inversion H0.
+          subst...
+          simpl.
+          assert (N.ftv t = N.ftv t2).
+          {
+            apply step_preserves_freevars with (t := t2); [reflexivity|assumption].
+          }
+          rewrite -> H.
+          apply SN_F.step_appR.
+          specialize (IHt2 t Hstep).
+          rewrite -> H in IHt2.
+          apply weaken_fv' with (ss := N.ftv t1) in IHt2.
+          assumption.
+
+      + unfold bind in H0.
+        destruct (namestep t1) eqn:Hstep in H0; try discriminate.
+        inversion H0.
+        subst...
+        simpl.
+        assert (N.ftv t = N.ftv t1).
+          {
+            apply step_preserves_freevars with (t := t1); [reflexivity|assumption].
+          }
+        rewrite -> H.
+        apply SN_F.step_appL.
+        specialize (IHt1 t Hstep).
+        rewrite -> H in IHt1.
+        apply weaken_fv'' with (ss := N.ftv t2) in IHt1.
+        assumption. *)
+Admitted.
+    
+    
+    
+
+Definition step_with_proof (t : N.term) : option {t' : N.term | SN_F.step (toDB' t (N.ftv t)) (toDB' t' (N.ftv t'))} :=
+  match namestep t with
+  | None => fun _ => None
+  | Some t' => fun Heq => (* Doing this function syntax thing to be able to use the equality hypothesis *)
+      let H_step := namestep_implies_step_nd t t' Heq in
+      Some (exist _ t' H_step)
+  end eq_refl.
+
+Fixpoint normalizer' (t : N.term) (H_sn : SN (toDB' t (N.ftv t))) : (forall t, option {t' | SN_F.step (toDB' t (N.ftv t)) (toDB' t' (N.ftv t'))}) -> N.term :=
+    fun stepper => match stepper t with
+    | None => t
+    | Some (exist _ t' H_step) => match H_sn with
+        | SNI f => normalizer' t' (f (toDB' t' (N.ftv t')) H_step) stepper
+        end
+end.
+
+(* Step t according to step' until we reach a value, i.e. normalise it*)
+Definition normalizer (t : N.term) (H_sn : SN (toDB' t (N.ftv t))) : N.term :=
+    normalizer' t H_sn step_with_proof.
